Moved generic definitions to core library.

src/Computation/ListComputations.v
@@ -1,7 +1,12 @@
-Require Import Coq.Sets.Ensembles
+Require Import
+        Coq.Arith.Arith
+        Coq.Sets.Ensembles
         Coq.Lists.List.
 
-Require Import Fiat.Computation.
+Require Import
+        Fiat.Common.List.ListFacts
+        Fiat.Common.DecideableEnsembles
+        Fiat.Computation.
 
 (* Operations on lists using computations. *)
 
@@ -47,6 +52,23 @@ Section ListComprehension.
       + subst; intuition.
   Qed.
 
+  Lemma refine_filtered_list
+    : forall (xs : list A)
+             (P : Ensemble A)
+             (P_dec : DecideableEnsemble P),
+      refine (build_FilteredList P xs)
+             (ret (filter dec xs)).
+  Proof.
+    unfold build_FilteredList; induction xs; intros.
+    - reflexivity.
+    - simpl; setoid_rewrite IHxs.
+      simplify with monad laws.
+      destruct (dec a) eqn: eq_dec_a;
+        [ setoid_rewrite dec_decides_P in eq_dec_a; refine pick val true |
+          setoid_rewrite Decides_false in eq_dec_a; refine pick val false ];
+        auto; simplify with monad laws; reflexivity.
+  Qed.
+
 End ListComprehension.
 
 Notation "⟦ x 'in' xs | P ⟧" :=
@@ -76,4 +98,42 @@ Section UpperBound.
     := elements' <- elements;
          ⟦ element in elements' | UpperBound elements' element ⟧.
 
+  Definition find_UpperBound (f : A -> nat) (ns : list A) : list A :=
+    let max := fold_right
+                 (fun n acc => max (f n) acc) O ns in
+    filter (fun n => NPeano.leb max (f n)) ns.
+
+  Lemma find_UpperBound_highest_length
+    : forall (f : A -> nat) ns n,
+      List.In n (find_UpperBound f ns) -> forall n', List.In n' ns -> (f n) >= (f n').
+  Proof.
+    unfold ge, find_UpperBound; intros.
+    apply filter_In in H; destruct H; apply NPeano.leb_le in H1.
+    rewrite <- H1; clear H1 H n.
+    apply fold_right_max_is_max; auto.
+  Qed.
+
 End UpperBound.
+
+Instance DecideableEnsembleUpperBound {A}
+         (f : A -> nat)
+         (ns : list A)
+  : DecideableEnsemble (UpperBound (fun a a' => f a >= f a') ns) :=
+  {| dec n := NPeano.leb (fold_right (fun n acc => max (f n) acc) O ns) (f n) |}.
+Proof.
+  unfold UpperBound, ge; intros; rewrite NPeano.leb_le; intuition.
+  - remember (f a); clear Heqn; subst; eapply le_trans;
+      [ apply fold_right_max_is_max; apply H0 | assumption ].
+  - eapply fold_right_higher_is_higher; eauto.
+Defined.
+
+Corollary refine_find_UpperBound {A}
+  : forall (f : A -> nat) ns,
+    refine (⟦ n in ns | UpperBound (fun a a' => f a >= f a') ns n ⟧)
+           (ret (find_UpperBound f ns)).
+Proof.
+  intros.
+  setoid_rewrite refine_ListComprehension_filtered_list.
+  setoid_rewrite refine_filtered_list with (P_dec := DecideableEnsembleUpperBound f ns).
+  reflexivity.
+Qed.
