src/Examples/DnsServer/DnsAutomation.v
@@ -1,79 +1,81 @@
-(*Require HintDbTactics.*)          (* plugin to pass a hint db to a tactic *)
-Require Import Coq.Vectors.Vector
+Require Import
+        Coq.Vectors.Vector
         Coq.Strings.Ascii
         Coq.Bool.Bool
         Coq.Bool.Bvector
         Coq.Lists.List.
 
-Require Import Fiat.QueryStructure.Automation.MasterPlan
+Require Import
+        Fiat.Computation.ListComputations
+        Fiat.QueryStructure.Automation.MasterPlan
         Fiat.QueryStructure.Implementation.DataStructures.BagADT.BagADT
         Fiat.QueryStructure.Automation.IndexSelection
         Fiat.QueryStructure.Specification.SearchTerms.ListPrefix
         Fiat.QueryStructure.Automation.SearchTerms.FindPrefixSearchTerms
         Fiat.QueryStructure.Automation.QSImplementation.
 
-Require Import Fiat.Examples.DnsServer.packet
-        Fiat.Examples.DnsServer.DnsSchema
+Require Import Fiat.Examples.DnsServer.Packet
+        Fiat.Examples.DnsServer.AuthoritativeDNSSchema
         Fiat.Examples.DnsServer.DnsLemmas.
 
 (* Process automation *)
 
-    Ltac invert_For_once :=
-      match goal with
-      | [ H : computes_to (Query_For _) _ |- _ ] =>
-        let H1 := fresh in
-        let H2 := fresh in
-        inversion H as [H1 H2]; inversion H2; clear H2
-      end.
+Ltac invert_For_once :=
+  match goal with
+  | [ H : computes_to (Query_For _) _ |- _ ] =>
+    let H1 := fresh in
+    let H2 := fresh in
+    inversion H as [H1 H2]; inversion H2; clear H2
+  end.
 
-      Ltac refine_under_bind' :=
-        setoid_rewrite refine_under_bind; [ higher_order_reflexivity |
-                                            let H := fresh in
-                                            intros a H; try invert_For_once ].
+Ltac refine_under_bind' :=
+  setoid_rewrite refine_under_bind; [ higher_order_reflexivity |
+                                      let H := fresh in
+                                      intros a H; try invert_For_once ].
 
-      Ltac refine_bind' :=
-        apply refine_bind; [ idtac | unfold pointwise_relation; intros; higher_order_reflexivity ].
+Ltac refine_bind' :=
+  apply refine_bind; [ idtac | unfold pointwise_relation; intros; higher_order_reflexivity ].
 
 (* ------------------------ *)
 (* AddData automation *)
 
-  Lemma eq_If_if {A}
+Lemma eq_If_if {A}
   : forall (c : bool) (t e : Comp A),
-      If c Then t Else e = if c then t else e.
-  Proof. intros. reflexivity. Qed.
+    If c Then t Else e = if c then t else e.
+Proof. intros. reflexivity. Qed.
 
-    (* don't rewrite inner If/Then/Else expressions *)
-    (* this can be made simpler by removing context[] to only do head matches *)
-    Ltac rewrite_if_head :=
-      match goal with
-      | [ |- context[ (refine (Bind _ (fun n => If_Then_Else _ _ _ )) _) ] ] =>
-        setoid_rewrite Bind_refine_If_Then_Else
-      end.
+(* don't rewrite inner If/Then/Else expressions *)
+(* this can be made simpler by removing context[] to only do head matches *)
+Ltac rewrite_if_head :=
+  match goal with
+  | [ |- context[ (refine (Bind _ (fun n => If_Then_Else _ _ _ )) _) ] ] =>
+    setoid_rewrite Bind_refine_If_Then_Else
+  end.
 
-      (* rewrite under bind the first time you can, then stop. otherwise fail *)
-      Ltac tac_under_bind tac :=
-        first [ tac |
-                (apply refine_under_bind; intros); tac_under_bind tac ].
+(* rewrite under bind the first time you can, then stop. otherwise fail *)
+Ltac tac_under_bind tac :=
+  first [ tac |
+          (apply refine_under_bind; intros); tac_under_bind tac ].
 
-      (* only succeed if all subgoals can be solved with tac.
+(* only succeed if all subgoals can be solved with tac.
 intended for use as setoid_rewrite_by *)
-      Ltac do_by tic tac :=
-        tic; [ | solve [tac] | .. | solve [tac] ].
+Ltac do_by tic tac :=
+  tic; [ | solve [tac] | .. | solve [tac] ].
 
 (* --------------------------- *)
 (* General, unified automation *)
 
-      (* tac is of form [first [ x1 | ... | xn]] *)
-      Ltac repeat_and_simplify tac :=
-        simpl in *;
-        try simplify with monad laws;
-        repeat (
-            try tac;
-            try simpl in *;
-            try simplify with monad laws
-          ).
+(* tac is of form [first [ x1 | ... | xn]] *)
+Ltac repeat_and_simplify tac :=
+  simpl in *;
+  try simplify with monad laws;
+  repeat (
+      try tac;
+      try simpl in *;
+      try simplify with monad laws
+    ).
 
-      (* For a tactic [top] that generates any number of subgoals, succeed only if tac (applied to each subgoal) EVENTUALLY makes progress on at least one of them [i.e. might need to drill twice in a row, the tac will work]. Then try cont again, keeping additional drilling/applying tac if it continues to make progress, until either tac fails everywhere or top fails.
+(* For a tactic [top] that generates any number of subgoals, succeed only if tac (applied to each subgoal) EVENTUALLY makes progress on at least one of them [i.e. might need to drill twice in a row, the tac will work]. Then try cont again, keeping additional drilling/applying tac if it continues to make progress, until either tac fails everywhere or top fails.
 
 Keep progress made in any of the subgoals (i.e. don't fail the whole thing because a sub-subgoal failed, even though progress was made in a subgoal).
 
@@ -81,8 +83,8 @@ Fails when top fails (fails iff tac never works on any subgoal) -- if top can lo
 
 Subgoals: even if everything fails in the other subgoal, the tactic will succeed if progress is made in the first subgoal, because the failure will be wrapped in a [try] *)
 
-      Ltac progress_subgoal top tac cont :=
-         top; (tac; try (cont ()) || (try (cont ()))).
+Ltac progress_subgoal top tac cont :=
+  top; (tac; try (cont ()) || (try (cont ()))).
 
 (* Succeeds:
 tac
@@ -104,64 +106,64 @@ top tac top (tac fails): keep progress up to tac, try cont
 
 All chains must end with tac, not top (because then there'd be no progress made under it) *)
 
-      (* ltac is call-by-value, so wrap the cont in a function *)
-      (* local definition in a_u_s *)
-      Ltac cont_fn top tac'' x :=
-        apply_under_subgoal top tac'' with
+(* ltac is call-by-value, so wrap the cont in a function *)
+(* local definition in a_u_s *)
+Ltac cont_fn top tac'' x :=
+  apply_under_subgoal top tac'' with
 
-      (* mutually recursive with progress_subgoal *)
-      (* calls top on each subgoal generated, which may generate more subgoals *)
-      (* fails when top fails in progress_subgoals *)
-      apply_under_subgoal top tac'' :=
-        progress_subgoal top tac'' ltac:(cont_fn top tac'').
+  (* mutually recursive with progress_subgoal *)
+  (* calls top on each subgoal generated, which may generate more subgoals *)
+  (* fails when top fails in progress_subgoals *)
+  apply_under_subgoal top tac'' :=
+    progress_subgoal top tac'' ltac:(cont_fn top tac'').
 
-      Theorem testthm : forall n, n = n + 0 + 0 + 0 + 0 + 0 + 0 + 0 + 0.
-      Proof.
-        intros.
-        assert (forall y, y + 0 = y) as tm. intros. omega.
-        specialize (tm n).
-        apply_under_subgoal ltac:(rewrite tm) ltac:(try reflexivity).
-      Qed.
+Theorem testthm : forall n, n = n + 0 + 0 + 0 + 0 + 0 + 0 + 0 + 0.
+Proof.
+  intros.
+  assert (forall y, y + 0 = y) as tm. intros. omega.
+  specialize (tm n).
+  apply_under_subgoal ltac:(rewrite tm) ltac:(try reflexivity).
+Qed.
 
-      (* Simplify. Try all the rewrites until none work.
+(* Simplify. Try all the rewrites until none work.
          If a rewrite works under a top, drill under the top and try all the rewrites until none work.
            (Do NOT drill down if no rewrite works. so: Try a drill, if failure for all rewrites, then backtrack, try a different trill. Difficult: there are multiple tops. )
          Keep doing this until none of the rewrites work at any layer of tops.
          Then, do the finishing tactics (eauto, reflexivity, various small lemmas).
          (These should all be done on all subgoals, keeping all progress made on each one.) *)
 
-      Ltac do_and_simplify tac :=
-        tac; (* no repeat *)
-        simpl in *;
-        try simplify with monad laws.
+Ltac do_and_simplify tac :=
+  tac; (* no repeat *)
+  simpl in *;
+  try simplify with monad laws.
 
-      Ltac srewrite_each_all :=
-        first [
-            (* Process *)
-            setoid_rewrite refine_pick_eq' |
-            rewrite (@refine_find_upperbound resourceRecord _ _) |
-            rewrite (@refine_decides_forall_In' _ _ _ _) |
-            rewrite refine_check_one_longest_prefix_s |
-            rewrite refine_if_If |
-            rewrite refine_check_one_longest_prefix_CNAME |
-            rewrite (@refine_filtered_list _ _ _ _) |
-            setoid_rewrite refine_bind_unit |
-            (* AddData *)
-            (* Why does adding these rewrites prevent other rewrites? *)
-            (* Should these be drills? *)
-            (* TODO messes up Process (only this one) *)
-            setoid_rewrite refine_If_Then_Else_Bind |
-            setoid_rewrite refine_count_constraint_broken |
-            setoid_rewrite refine_count_constraint_broken' |
-            setoid_rewrite refine_Count |
-            do_by
-              ltac:(setoid_rewrite refine_subcheck_to_filter) ltac:(eauto with typeclass_instances) |
-            (* set_evars needed because otherwise it rewrites forever in an evar *)
-            (* hacky way to revert outer If to if *)
-            try (set_evars; rewrite eq_If_if);
-              set_evars; rewrite clear_nested_if by apply filter_nil_is_nil
-           (* set_evars; setoid_rewrite refine_if_If *) (* can be done later *)
-          ].
+Ltac srewrite_each_all :=
+  first [
+      (* Process *)
+      setoid_rewrite refine_pick_eq' |
+      rewrite (@refine_find_UpperBound resourceRecord _ _) |
+      rewrite (@refine_decides_forall_In' _ _ _ _) |
+      rewrite refine_check_one_longest_prefix_s |
+      rewrite refine_if_If |
+      rewrite refine_check_one_longest_prefix_CNAME |
+      rewrite (@refine_filtered_list _ _ _ _) |
+      setoid_rewrite refine_bind_unit |
+      (* AddData *)
+      (* Why does adding these rewrites prevent other rewrites? *)
+      (* Should these be drills? *)
+      (* TODO messes up Process (only this one) *)
+      setoid_rewrite refine_If_Then_Else_Bind |
+      setoid_rewrite refine_count_constraint_broken |
+      setoid_rewrite refine_count_constraint_broken' |
+      setoid_rewrite refine_Count |
+      do_by
+        ltac:(setoid_rewrite refine_subcheck_to_filter) ltac:(eauto with typeclass_instances) |
+      (* set_evars needed because otherwise it rewrites forever in an evar *)
+      (* hacky way to revert outer If to if *)
+      try (set_evars; rewrite eq_If_if);
+      set_evars; rewrite clear_nested_if by apply filter_nil_is_nil
+                                                  (* set_evars; setoid_rewrite refine_if_If *) (* can be done later *)
+    ].
 
 Ltac subst_all' :=
   repeat match goal with H : _ |- _ => subst H end.
@@ -187,9 +189,9 @@ Ltac doAny srewrite_fn drills_fn finish_fn :=
   let repeat_srewrite_fn := repeat_and_simplify srewrite_fn in
   let anyDrill_fn := do_and_simplify drills_fn in
   let repeat_finish_fn := repeat_and_simplify finish_fn in
-        try repeat_srewrite_fn;
-        apply_under_subgoal ltac:(anyDrill_fn) ltac:(repeat_srewrite_fn);
-        repeat_finish_fn.
+  try repeat_srewrite_fn;
+  apply_under_subgoal ltac:(anyDrill_fn) ltac:(repeat_srewrite_fn);
+  repeat_finish_fn.
 
 Ltac doAnyAll := doAny srewrite_each_all drills_each_all finish_each_all.
 (* combinator libraries similar to (a, b, c) (d, e, f) ~> (a || d, b || e, c || f)
@@ -236,23 +238,23 @@ Ltac hone_Dns :=
                                                                          let attrlist' := eval compute in (PickIndexes (CountAttributes' attrlist)) in makeIndex attrlist')).
 
 Ltac srewrite_each_all ::=
-    first
-  [ rewrite refine_pick_eq'
-  | rewrite (refine_find_upperbound _ _)
-  | rewrite (refine_decides_forall_In' _ _)
-  | rewrite refine_check_one_longest_prefix_s
-  | rewrite refine_if_If
-  | rewrite refine_check_one_longest_prefix_CNAME
-  | rewrite (refine_filtered_list _ _)
-  | rewrite refine_bind_unit
-  | rewrite refine_If_Then_Else_Bind
-  | rewrite refine_count_constraint_broken
-  | rewrite refine_count_constraint_broken'
-  | rewrite refine_Count
-  | do_by ltac:(rewrite refine_subcheck_to_filter)
-     ltac:(eauto  with typeclass_instances)
-  | try (set_evars; rewrite eq_If_if); set_evars;
-     rewrite clear_nested_if by apply filter_nil_is_nil ].
+     first
+     [ rewrite refine_pick_eq'
+     | rewrite (refine_find_UpperBound _ _)
+     | rewrite (refine_decides_forall_In' _ _)
+     | rewrite refine_check_one_longest_prefix_s
+     | rewrite refine_if_If
+     | rewrite refine_check_one_longest_prefix_CNAME
+     | rewrite (refine_filtered_list _ _)
+     | rewrite refine_bind_unit
+     | rewrite refine_If_Then_Else_Bind
+     | rewrite refine_count_constraint_broken
+     | rewrite refine_count_constraint_broken'
+     | rewrite refine_Count
+     | do_by ltac:(rewrite refine_subcheck_to_filter)
+                    ltac:(eauto  with typeclass_instances)
+     | try (set_evars; rewrite eq_If_if); set_evars;
+       rewrite clear_nested_if by apply filter_nil_is_nil ].
 
 Ltac FullySharpenQueryStructure'' qs_schema Index :=
   let DelegateSigs := constr:(@Build_IndexedQueryStructure_Impl_Sigs _ (qschemaSchemas qs_schema) Index) in
@@ -302,10 +304,10 @@ Ltac FullySharpenQueryStructure'' qs_schema Index :=
                                                                Iterate_Dep_Type_BoundedIndex
                                                                  (fun idx =>
                                                                     @refineConstructor _
-                                                                      (cRep' DelegateReps) (cAbsR' _ _ ValidImpls)
-                                                  (consDom (Vector.nth consSigs idx))
-                                                  (getConsDef consDefs idx)
-                                                  (ComputationalADT.LiftcConstructor _ _ (ith  (cCons DelegateReps DelegateImpls) idx))))
+                                                                                       (cRep' DelegateReps) (cAbsR' _ _ ValidImpls)
+                                                                                       (consDom (Vector.nth consSigs idx))
+                                                                                       (getConsDef consDefs idx)
+                                                                                       (ComputationalADT.LiftcConstructor _ _ (ith  (cCons DelegateReps DelegateImpls) idx))))
                                                            * (forall
                                                                  (DelegateReps : Fin.t (numRawQSschemaSchemas qs_schema) -> Type)
                                                                  (DelegateImpls : forall idx,
@@ -323,84 +325,84 @@ Ltac FullySharpenQueryStructure'' qs_schema Index :=
                                                                         (methCod (Vector.nth methSigs idx))
                                                                         (getMethDef methDefs idx)
                                                                         (ComputationalADT.LiftcMethod (ith (cMeths DelegateReps DelegateImpls) idx))))) as ValidRefinements;
-                                                      [ |
-                                                        pose proof (@Notation_Friendly_SharpenFully'
-                                                                      _
-                                                                      _
-                                                                      _
-                                                                      consSigs
-                                                                      methSigs
-                                                                      consDefs
-                                                                      methDefs
-                                                                      _
-                                                                      DelegateSigs
-                                                                      cRep'
-                                                                      cCons
-                                                                      cMeths
-                                                                      DelegateSpecs
-                                                                      cAbsR'
-                                                                      (fst ValidRefinements)
-                                                                      (snd ValidRefinements))
-                                                          as FullySharpenedImpl
-                                                        ; clear ValidRefinements ] ))
+                                                        [ |
+                                                          pose proof (@Notation_Friendly_SharpenFully'
+                                                                        _
+                                                                        _
+                                                                        _
+                                                                        consSigs
+                                                                        methSigs
+                                                                        consDefs
+                                                                        methDefs
+                                                                        _
+                                                                        DelegateSigs
+                                                                        cRep'
+                                                                        cCons
+                                                                        cMeths
+                                                                        DelegateSpecs
+                                                                        cAbsR'
+                                                                        (fst ValidRefinements)
+                                                                        (snd ValidRefinements))
+                                                            as FullySharpenedImpl
+                                                          ; clear ValidRefinements ] ))
   end;
-    [ simpl; intros; split;
-      [ repeat split; intros; try exact tt;
-        try (etransitivity;
-             [eapply (@Initialize_IndexedQueryStructureImpls_AbsR qs_schema Index)
-             | ];
-             cbv beta;
-             unfold Initialize_IndexedQueryStructureImpls',
-             CallBagImplConstructor; simpl;
-             higher_order_reflexivity
-            )
-      | repeat split; intros; try exact tt;
-        try implement_bag_methods
-      ] | ];
-    simpl in FullySharpenedImpl;
-    fold_string_hyps_in FullySharpenedImpl;
-    fold_heading_hyps_in FullySharpenedImpl;
-    pose_SearchUpdateTerms_in FullySharpenedImpl;
-    pose_search_term_in FullySharpenedImpl;
-    let impl := fresh "impl" in
-    match type of FullySharpenedImpl with
-      @FullySharpenedUnderDelegates _ _ ?Impl =>
-      set (impl := Impl) in *
-    end;
-      cbv beta in *; simpl in impl;
-      let impl' :=
-          match goal with
-            |- @FullySharpenedUnderDelegates _ _ ?Impl => Impl
-          end in
-      (* Not having to worry about re-typing the body during zeta-expansion
+  [ simpl; intros; split;
+    [ repeat split; intros; try exact tt;
+      try (etransitivity;
+           [eapply (@Initialize_IndexedQueryStructureImpls_AbsR qs_schema Index)
+           | ];
+           cbv beta;
+           unfold Initialize_IndexedQueryStructureImpls',
+           CallBagImplConstructor; simpl;
+           higher_order_reflexivity
+          )
+    | repeat split; intros; try exact tt;
+      try implement_bag_methods
+    ] | ];
+  simpl in FullySharpenedImpl;
+  fold_string_hyps_in FullySharpenedImpl;
+  fold_heading_hyps_in FullySharpenedImpl;
+  pose_SearchUpdateTerms_in FullySharpenedImpl;
+  pose_search_term_in FullySharpenedImpl;
+  let impl := fresh "impl" in
+  match type of FullySharpenedImpl with
+    @FullySharpenedUnderDelegates _ _ ?Impl =>
+    set (impl := Impl) in *
+  end;
+  cbv beta in *; simpl in impl;
+  let impl' :=
+      match goal with
+        |- @FullySharpenedUnderDelegates _ _ ?Impl => Impl
+      end in
+  (* Not having to worry about re-typing the body during zeta-expansion
      yields a 30x speedup.
-       *)
-      assert (True) by
-          (clear FullySharpenedImpl; zeta_expand_all impl; unify impl impl'; econstructor);
-        exact FullySharpenedImpl.
+   *)
+  assert (True) by
+      (clear FullySharpenedImpl; zeta_expand_all impl; unify impl impl'; econstructor);
+  exact FullySharpenedImpl.
 
 Ltac Finish_Master BuildEarlyBag BuildLastBag :=
-    eapply FullySharpened_Finish;
-    [pose_headings_all;
-      match goal with
-      | |- appcontext[ @BuildADT (IndexedQueryStructure ?Schema ?Indexes) ] =>
-        FullySharpenQueryStructure'' Schema Indexes
-      end
-    | simpl; pose_string_ids; pose_headings_all;
-      pose_search_term;  pose_SearchUpdateTerms;
-      match goal with
-        |- context [ @Build_IndexedQueryStructure_Impl_Sigs _ ?indices ?SearchTerms _] => try unfold SearchTerms
-      end;
-      BuildQSIndexedBags' BuildEarlyBag BuildLastBag
-    | cbv zeta; pose_string_ids; pose_headings_all;
-      pose_search_term;  pose_SearchUpdateTerms;
-      simpl Sharpened_Implementation;
-      unfold
-        Update_Build_IndexedQueryStructure_Impl_cRep,
-      Join_Comp_Lists',
-      GetIndexedQueryStructureRelation,
-      GetAttributeRaw; simpl;
-      higher_order_reflexivityT ].
+  eapply FullySharpened_Finish;
+  [pose_headings_all;
+   match goal with
+   | |- appcontext[ @BuildADT (IndexedQueryStructure ?Schema ?Indexes) ] =>
+     FullySharpenQueryStructure'' Schema Indexes
+   end
+  | simpl; pose_string_ids; pose_headings_all;
+    pose_search_term;  pose_SearchUpdateTerms;
+    match goal with
+      |- context [ @Build_IndexedQueryStructure_Impl_Sigs _ ?indices ?SearchTerms _] => try unfold SearchTerms
+    end;
+    BuildQSIndexedBags' BuildEarlyBag BuildLastBag
+  | cbv zeta; pose_string_ids; pose_headings_all;
+    pose_search_term;  pose_SearchUpdateTerms;
+    simpl Sharpened_Implementation;
+    unfold
+      Update_Build_IndexedQueryStructure_Impl_cRep,
+    Join_Comp_Lists',
+    GetIndexedQueryStructureRelation,
+    GetAttributeRaw; simpl;
+    higher_order_reflexivityT ].
 
 Ltac Focused_refine_TopMost_Query :=
   match goal with
@@ -409,8 +411,8 @@ Ltac Focused_refine_TopMost_Query :=
              ltac:(fun body' =>
                      let refine_body' := fresh in
                      assert (refine body body') as refine_body';
-                   [ |
-                     setoid_rewrite refine_body';
+                     [ |
+                       setoid_rewrite refine_body';
                        setoid_rewrite (@refine_For_List ResultT body') at 1;
                        setoid_rewrite (@refine_Count ResultT body') at 1;
                        clear refine_body' ] )
@@ -420,8 +422,8 @@ Ltac Focused_refine_TopMost_Query :=
              ltac:(fun body' =>
                      let refine_body' := fresh in
                      assert (refine body body') as refine_body';
-                   [ |
-                     setoid_rewrite refine_body';
+                     [ |
+                       setoid_rewrite refine_body';
                        setoid_rewrite (@refine_For_List ResultT body') at 1;
                        setoid_rewrite (@refine_MaxN body') at 1;
                        clear refine_body' ] )
@@ -431,8 +433,8 @@ Ltac Focused_refine_TopMost_Query :=
              ltac:(fun body' =>
                      let refine_body' := fresh in
                      assert (refine body body') as refine_body';
-                   [ |
-                     setoid_rewrite refine_body';
+                     [ |
+                       setoid_rewrite refine_body';
                        setoid_rewrite (@refine_For_List ResultT body') at 1;
                        setoid_rewrite (@refine_SumN body') at 1;
                        clear refine_body' ] )
@@ -442,8 +444,8 @@ Ltac Focused_refine_TopMost_Query :=
              ltac:(fun body' =>
                      let refine_body' := fresh in
                      assert (refine body body') as refine_body';
-                   [ |
-                     setoid_rewrite refine_body';
+                     [ |
+                       setoid_rewrite refine_body';
                        setoid_rewrite (@refine_For_List ResultT body') at 1;
                        setoid_rewrite (@refine_MaxZ body') at 1;
                        clear refine_body' ] )
@@ -453,8 +455,8 @@ Ltac Focused_refine_TopMost_Query :=
              ltac:(fun body' =>
                      let refine_body' := fresh in
                      assert (refine body body') as refine_body';
-                   [ |
-                     setoid_rewrite refine_body';
+                     [ |
+                       setoid_rewrite refine_body';
                        setoid_rewrite (@refine_For_List ResultT body') at 1;
                        setoid_rewrite (@refine_SumZ body') at 1;
                        clear refine_body' ] )
@@ -464,8 +466,8 @@ Ltac Focused_refine_TopMost_Query :=
              ltac:(fun body' =>
                      let refine_body' := fresh in
                      assert (refine body body') as refine_body';
-                   [ |
-                     setoid_rewrite refine_body';
+                     [ |
+                       setoid_rewrite refine_body';
                        setoid_rewrite (@refine_For_List ResultT body') at 1;
                        setoid_rewrite (@refine_Max body') at 1;
                        clear refine_body' ] )
@@ -475,8 +477,8 @@ Ltac Focused_refine_TopMost_Query :=
              ltac:(fun body' =>
                      let refine_body' := fresh in
                      assert (refine body body') as refine_body';
-                   [ |
-                     setoid_rewrite refine_body';
+                     [ |
+                       setoid_rewrite refine_body';
                        setoid_rewrite (@refine_For_List ResultT body') at 1;
                        setoid_rewrite (@refine_Sum body') at 1;
                        clear refine_body' ] )
@@ -486,8 +488,8 @@ Ltac Focused_refine_TopMost_Query :=
              ltac:(fun body' =>
                      let refine_body' := fresh in
                      assert (refine body body') as refine_body';
-                   [ |
-                     setoid_rewrite refine_body';
+                     [ |
+                       setoid_rewrite refine_body';
                        setoid_rewrite (@refine_For_List ResultT body') at 1;
                        clear refine_body' ] )
 
@@ -512,7 +514,7 @@ Ltac implement_TopMost_Query CreateTerm EarlyIndex LastIndex
     ltac:(find_simple_search_term CreateTerm EarlyIndex LastIndex)
            ltac:(find_simple_search_term_dep makeClause_dep EarlyIndex_dep LastIndex_dep).
 
- Ltac implement_insert' CreateTerm EarlyIndex LastIndex
+Ltac implement_insert' CreateTerm EarlyIndex LastIndex
      makeClause_dep EarlyIndex_dep LastIndex_dep :=
   first
     [simplify with monad laws; simpl
@@ -529,7 +531,7 @@ Ltac implement_TopMost_Query CreateTerm EarlyIndex LastIndex
         |- context[Pick (fun idx => UnConstrFreshIdx (GetUnConstrRelation ?r_o ?Ridx) idx)] =>
         let freshIdx := fresh in
         destruct (exists_UnConstrFreshIdx H Ridx) as [? freshIdx];
-          setoid_rewrite (refine_Pick_UnConstrFreshIdx H Ridx freshIdx)
+        setoid_rewrite (refine_Pick_UnConstrFreshIdx H Ridx freshIdx)
       end
     | implement_QSDeletedTuples ltac:(find_simple_search_term
                                         CreateTerm EarlyIndex LastIndex)
@@ -537,7 +539,7 @@ Ltac implement_TopMost_Query CreateTerm EarlyIndex LastIndex
                               makeClause_dep EarlyIndex_dep LastIndex_dep
     | implement_Pick_DelegateToBag_AbsR ].
 
- Ltac master_implement_drill CreateTerm EarlyIndex LastIndex :=
+Ltac master_implement_drill CreateTerm EarlyIndex LastIndex :=
   subst_refine_evar;
   first
     [ eapply refine_BagADT_QSInsert'; try eassumption; intros
@@ -551,49 +553,49 @@ Ltac implement_TopMost_Query CreateTerm EarlyIndex LastIndex
     | eapply refine_If_Opt_Then_Else;
       [intro; set_refine_evar | set_refine_evar ] ].
 
- Ltac implement_insert'' :=
-        implement_insert'
-               ltac:(CombineCase5 PrefixIndexUse EqIndexUse)
-                      ltac:(CombineCase10 createEarlyPrefixTerm createEarlyEqualityTerm)
-                             ltac:(CombineCase7 createLastPrefixTerm createLastEqualityTerm)
-                                    ltac:(CombineCase7 PrefixIndexUse_dep EqIndexUse_dep)
-                                           ltac:(CombineCase11 createEarlyPrefixTerm_dep createEarlyEqualityTerm_dep)
-                                                  ltac:(CombineCase8 createLastPrefixTerm_dep createLastEqualityTerm_dep).
+Ltac implement_insert'' :=
+  implement_insert'
+    ltac:(CombineCase5 PrefixIndexUse EqIndexUse)
+           ltac:(CombineCase10 createEarlyPrefixTerm createEarlyEqualityTerm)
+                  ltac:(CombineCase7 createLastPrefixTerm createLastEqualityTerm)
+                         ltac:(CombineCase7 PrefixIndexUse_dep EqIndexUse_dep)
+                                ltac:(CombineCase11 createEarlyPrefixTerm_dep createEarlyEqualityTerm_dep)
+                                       ltac:(CombineCase8 createLastPrefixTerm_dep createLastEqualityTerm_dep).
 
- Ltac doOne srewrite_fn drills_fn finish_fn :=
+Ltac doOne srewrite_fn drills_fn finish_fn :=
   first [srewrite_fn | drills_fn | finish_fn].
 
- Ltac drop_constraintsfrom_DNS :=
+Ltac drop_constraintsfrom_DNS :=
   eapply SharpenStep;
   [ match goal with
-        |- context [ @BuildADT (QueryStructure ?Rep) _ _ _ _ _ _] =>
-        eapply refineADT_BuildADT_Rep_refine_All with (AbsR := @DropQSConstraints_AbsR Rep);
-          [ repeat (first [eapply refine_Constructors_nil
-                          | eapply refine_Constructors_cons;
-                            [ simpl; intros;
-                              match goal with
-                              | |- refine _ (?E _ _ _ _) => let H := fresh in set (H := E)
-                              | |- refine _ (?E _ _ _) => let H := fresh in set (H := E)
-                              | |- refine _ (?E _ _) => let H := fresh in set (H := E)
-                              | |- refine _ (?E _) => let H := fresh in set (H := E)
-                              | |- refine _ (?E) => let H := fresh in set (H := E)
-                              | _ => idtac
-                              end;
-                              (* Drop constraints from empty *)
-                              try apply Constructor_DropQSConstraints;
-                              cbv delta [GetAttribute] beta; simpl
-                            | ] ])
-          | repeat (first [eapply refine_Methods_nil
-                          | eapply refine_Methods_cons;
-                            [ simpl; intros;
-                              match goal with
-                              | |- refine _ (?E _ _ _ _) => let H := fresh in set (H := E)
-                              | |- refine _ (?E _ _ _) => let H := fresh in set (H := E)
-                              | |- refine _ (?E _ _) => let H := fresh in set (H := E)
-                              | |- refine _ (?E _) => let H := fresh in set (H := E)
-                              | |- refine _ (?E) => let H := fresh in set (H := E)
-                              | _ => idtac
-                              end;
-                              cbv delta [GetAttribute] beta; simpl | ]
-                          ])]
+      |- context [ @BuildADT (QueryStructure ?Rep) _ _ _ _ _ _] =>
+      eapply refineADT_BuildADT_Rep_refine_All with (AbsR := @DropQSConstraints_AbsR Rep);
+      [ repeat (first [eapply refine_Constructors_nil
+                      | eapply refine_Constructors_cons;
+                        [ simpl; intros;
+                          match goal with
+                          | |- refine _ (?E _ _ _ _) => let H := fresh in set (H := E)
+                          | |- refine _ (?E _ _ _) => let H := fresh in set (H := E)
+                          | |- refine _ (?E _ _) => let H := fresh in set (H := E)
+                          | |- refine _ (?E _) => let H := fresh in set (H := E)
+                          | |- refine _ (?E) => let H := fresh in set (H := E)
+                          | _ => idtac
+                          end;
+                          (* Drop constraints from empty *)
+                          try apply Constructor_DropQSConstraints;
+                          cbv delta [GetAttribute] beta; simpl
+                        | ] ])
+      | repeat (first [eapply refine_Methods_nil
+                      | eapply refine_Methods_cons;
+                        [ simpl; intros;
+                          match goal with
+                          | |- refine _ (?E _ _ _ _) => let H := fresh in set (H := E)
+                          | |- refine _ (?E _ _ _) => let H := fresh in set (H := E)
+                          | |- refine _ (?E _ _) => let H := fresh in set (H := E)
+                          | |- refine _ (?E _) => let H := fresh in set (H := E)
+                          | |- refine _ (?E) => let H := fresh in set (H := E)
+                          | _ => idtac
+                          end;
+                          cbv delta [GetAttribute] beta; simpl | ]
+      ])]
     end | ].
