src/Examples/DnsServer/DnsLemmas.v
@@ -4,18 +4,20 @@ Require Import Coq.Vectors.Vector
         Coq.Bool.Bvector
         Coq.Lists.List.
 
-Require Import Fiat.QueryStructure.Automation.AutoDB
+Require Import
+        Fiat.Computation.ListComputations
+        Fiat.QueryStructure.Automation.AutoDB
         Fiat.QueryStructure.Implementation.DataStructures.BagADT.BagADT
         Fiat.QueryStructure.Automation.IndexSelection
         Fiat.QueryStructure.Specification.SearchTerms.ListPrefix
         Fiat.QueryStructure.Automation.SearchTerms.FindPrefixSearchTerms
         Fiat.QueryStructure.Automation.QSImplementation
-        Fiat.Examples.DnsServer.Packet.
+        Fiat.Examples.DnsServer.Packet
+        Fiat.Examples.DnsServer.AuthoritativeDNSSchema.
 
 Open Scope list_scope.
 
-Definition is_empty {A} (l : list A) :=
-  match l with nil => true | _ => false end.
+
 (* Refinement lemmas *)
 
 (* First, lemmas that help with honing the AddData method in DnsManual. They're related to implementing the data constraint (on DnsSchema) as a query. *)
@@ -29,8 +31,8 @@ Lemma refine_not_CNAME__independent :
     -> refine {b |
                decides b
                        (forall tup' : IndexedTuple,
-                          R tup' ->
-                          n!sNAME= (indexedElement tup')!sNAME -> n!sTYPE <> CNAME)}
+                           R tup' ->
+                           n!sNAME= (indexedElement tup')!sNAME -> n!sTYPE <> CNAME)}
 
               (ret true).
 Proof.
@@ -46,21 +48,21 @@ Lemma refine_is_CNAME__forall_to_exists :
     -> refine {b |
                decides b
                        (forall tup' : IndexedTuple,
-                          R tup' ->
-                          n!sNAME = (indexedElement tup')!sNAME -> n!sTYPE <> CNAME)}
+                           R tup' ->
+                           n!sNAME = (indexedElement tup')!sNAME -> n!sTYPE <> CNAME)}
               (b <- {b |
                      decides b
                              (exists tup' : IndexedTuple,
-                                R tup' /\
-                                n!sNAME = (indexedElement tup')!sNAME)};
-               ret (negb b)).
+                                 R tup' /\
+                                 n!sNAME = (indexedElement tup')!sNAME)};
+                 ret (negb b)).
 Proof.
-   repeat match goal with
-    | _ : _ ↝ _ |- _ => computes_to_inv
-    | _ : negb ?v = _ |- _ => destruct v; simpl in *; subst
-    | _ : ex _ |- _ => destruct_ex
-    | _ => progress first [ intro | computes_to_econstructor | simpl; intuition; eauto ]
-          end.
+  repeat match goal with
+         | _ : _ ↝ _ |- _ => computes_to_inv
+         | _ : negb ?v = _ |- _ => destruct v; simpl in *; subst
+         | _ : ex _ |- _ => destruct_ex
+         | _ => progress first [ intro | computes_to_econstructor | simpl; intuition; eauto ]
+         end.
 Qed.
 
 (* very similar to refine_is_CNAME__forall_to_exists;
@@ -70,22 +72,22 @@ Lemma refine_forall_to_exists :
     refine {b |
             decides b
                     (forall tup' : IndexedTuple,
-                       R tup' ->
-                       (indexedElement tup')!sNAME = n!sNAME
-                       -> (indexedElement tup')!sTYPE <> CNAME)}
+                        R tup' ->
+                        (indexedElement tup')!sNAME = n!sNAME
+                        -> (indexedElement tup')!sTYPE <> CNAME)}
            (b <- {b |
                   decides b
                           (exists tup' : IndexedTuple,
-                             R tup' /\
-                             n!sNAME = (indexedElement tup')!sNAME
-                             /\ (indexedElement tup')!sTYPE = CNAME)};
-            ret (negb b)).
+                              R tup' /\
+                              n!sNAME = (indexedElement tup')!sNAME
+                              /\ (indexedElement tup')!sTYPE = CNAME)};
+              ret (negb b)).
 Proof.                          (* same proof as refine_is_CNAME__forall_to_exists *)
   repeat match goal with
-    | _ : _ ↝ _ |- _ => computes_to_inv
-    | _ : negb ?v = _ |- _ => destruct v; simpl in *; subst
-    | _ : ex _ |- _ => destruct_ex
-    | _ => progress first [ intro | computes_to_econstructor | simpl; intuition; eauto ]
+         | _ : _ ↝ _ |- _ => computes_to_inv
+         | _ : negb ?v = _ |- _ => destruct v; simpl in *; subst
+         | _ : ex _ |- _ => destruct_ex
+         | _ => progress first [ intro | computes_to_econstructor | simpl; intuition; eauto ]
          end.
 Qed.
 
@@ -96,48 +98,48 @@ Lemma refine_count_constraint_broken :
   forall (n : resourceRecord) (r : UnConstrQueryStructure DnsSchema),
     refine {b |
             decides b
-                    (forall tup' : @IndexedRawTuple (GetHeading DnsSchema sCOLLECTIONS),
-                       (r!sCOLLECTIONS)%QueryImpl tup' ->
-                       n!sNAME = (indexedElement tup')!sNAME -> n!sTYPE <> CNAME)}
+                    (forall tup' : @IndexedRawTuple (GetHeading DnsSchema sRRecords),
+                        (r!sRRecords)%QueryImpl tup' ->
+                        n!sNAME = (indexedElement tup')!sNAME -> n!sTYPE <> CNAME)}
            (If (beq_RRecordType n!sTYPE CNAME)
                Then count <- Count
-               For (tup in r!sCOLLECTIONS)
+               For (tup in r!sRRecords)
                (Where (n!sNAME = tup!sNAME)
                       Return tup )%QueryImpl;
-    ret (beq_nat count 0) Else ret true).
+              ret (beq_nat count 0) Else ret true).
 Proof.
   (* intros; setoid_rewrite refine_pick_decides at 1. *)
   (* - Check refine_is_CNAME__forall_to_exists. apply refine_is_CNAME__forall_to_exists. *)
   (* [ | apply refine_is_CNAME__forall_to_exists | apply refine_not_CNAME__independent ]. *)
 
   intros; setoid_rewrite refine_pick_decides at 1;
-  [ | apply refine_is_CNAME__forall_to_exists | apply refine_not_CNAME__independent ].
+    [ | apply refine_is_CNAME__forall_to_exists | apply refine_not_CNAME__independent ].
   (* refine existence check into query. *)
 
   match goal with
-      |- context[{b | decides b
-                              (exists tup : @IndexedTuple ?heading,
-                                 (@GetUnConstrRelationBnd ?qs_schema ?qs ?tbl tup /\ @?P tup))}]
-      =>
-      let H1 := fresh in
-      let H2 := fresh in
-      makeEvar (Ensemble (@Tuple heading))
-               ltac:(fun P' => assert (Same_set (@IndexedTuple heading) (fun t => P' (indexedElement t)) P) as H1;
-                     [unfold Same_set, Included, Ensembles.In;
-                       split; [intros x H; pattern (indexedElement x);
-                               match goal with
-                                   |- ?P'' (indexedElement x) => unify P' P'';
-                                     simpl; eauto
-                               end
-                              | eauto]
-                     |
-                     assert (DecideableEnsemble P') as H2;
-                       [ simpl; eauto with typeclass_instances (* Discharge DecideableEnsemble w/ intances. *)
-                       | setoid_rewrite (@refine_constraint_check_into_query' qs_schema (ibound (indexb tbl)) qs P P' H2 H1); clear H2 H1 ] ]) end.
+    |- context[{b | decides b
+                            (exists tup : @IndexedTuple ?heading,
+                                (@GetUnConstrRelationBnd ?qs_schema ?qs ?tbl tup /\ @?P tup))}]
+    =>
+    let H1 := fresh in
+    let H2 := fresh in
+    makeEvar (Ensemble (@Tuple heading))
+             ltac:(fun P' => assert (Same_set (@IndexedTuple heading) (fun t => P' (indexedElement t)) P) as H1;
+                             [unfold Same_set, Included, Ensembles.In;
+                              split; [intros x H; pattern (indexedElement x);
+                                      match goal with
+                                        |- ?P'' (indexedElement x) => unify P' P'';
+                                                                      simpl; eauto
+                                      end
+                                     | eauto]
+                             |
+                             assert (DecideableEnsemble P') as H2;
+                             [ simpl; eauto with typeclass_instances (* Discharge DecideableEnsemble w/ intances. *)
+                             | setoid_rewrite (@refine_constraint_check_into_query' qs_schema (ibound (indexb tbl)) qs P P' H2 H1); clear H2 H1 ] ]) end.
   remember n!sTYPE; refine pick val (beq_RRecordType d CNAME); subst;
-  [ | case_eq (beq_RRecordType n!sTYPE CNAME); intros;
-      rewrite <- beq_RRecordType_dec in H; find_if_inside;
-      unfold not; simpl in *; try congruence ].
+    [ | case_eq (beq_RRecordType n!sTYPE CNAME); intros;
+        rewrite <- beq_RRecordType_dec in H; find_if_inside;
+        unfold not; simpl in *; try congruence ].
   intros; simplify with monad laws; simpl.
   autorewrite with monad laws.
   setoid_rewrite negb_involutive.
@@ -153,9 +155,9 @@ uses P' decision procedure invisibly in DecideableEnsembles.dec by the magic of 
 (try Set Printing Implicit) *)
 
 Lemma refine_subcheck_to_filter {heading}
-: forall (R : Ensemble (@IndexedTuple heading))
-         (P : Ensemble Tuple) (P_dec : DecideableEnsemble P)
-         (l : list Tuple),
+  : forall (R : Ensemble (@IndexedTuple heading))
+           (P : Ensemble Tuple) (P_dec : DecideableEnsemble P)
+           (l : list Tuple),
     For (QueryResultComp
            R
            (fun tup => Where (P tup) (* tuple is in P *)
@@ -186,14 +188,14 @@ Proof.
         intuition eauto. eauto.
         apply eq_ret_compute; destruct (@dec _ P P_dec a) eqn: dec__a.
         apply dec_decides_P in dec__a; apply H in dec__a;
-        computes_to_inv; subst; simpl; rewrite dec_a'; reflexivity.
+          computes_to_inv; subst; simpl; rewrite dec_a'; reflexivity.
         apply Decides_false in dec__a; apply H0 in dec__a; subst; reflexivity.
       * pose proof dec_a as dec_a'; apply Decides_false in dec_a.
         repeat computes_to_inv; repeat computes_to_econstructor.
         intuition eauto. eauto.
         apply eq_ret_compute; destruct (@dec _ P P_dec a) eqn: dec__a.
         apply dec_decides_P in dec__a; apply H in dec__a;
-        computes_to_inv; subst; simpl; rewrite dec_a'; reflexivity.
+          computes_to_inv; subst; simpl; rewrite dec_a'; reflexivity.
         apply Decides_false in dec__a; apply H0 in dec__a; subst; reflexivity.
   - refine pick val _; auto; subst.
     apply List.ListMorphisms.filter_permutation_morphism; [ reflexivity | assumption ].
@@ -211,12 +213,12 @@ Lemma refine_count_constraint_broken :
   forall (n : resourceRecord) (r : UnConstrQueryStructure DnsSchema),
     refine {b |
             decides b
-                    (forall tup' : @IndexedTuple (GetHeading DnsSchema sCOLLECTIONS),
-                       (r!sCOLLECTIONS)%QueryImpl tup' ->
+                    (forall tup' : @IndexedTuple (GetHeading DnsSchema sRRecords),
+                       (r!sRRecords)%QueryImpl tup' ->
                        n!sNAME = (indexedElement tup')!sNAME -> n!sTYPE <> CNAME)}
            (If (beq_RRecordType n!sTYPE CNAME)
                Then count <- Count
-               For (UnConstrQuery_In r ``(sCOLLECTIONS)
+               For (UnConstrQuery_In r ``(sRRecords)
                                      (fun tup : Tuple =>
                                         Where (n!sNAME = tup!sNAME)
                                               Return tup ));
@@ -254,23 +256,23 @@ Proof.
   setoid_rewrite negb_involutive.
   reflexivity.
 Qed.
-*)
+ *)
 
 (* uses refine_forall_to_exists; refines x2 in AddData
 very similar to refine_count_constraint_broken; comments below are relative to refine_count_constraint_broken *)
 
 Definition bCOLLECTIONS : Fin.t _ :=
   ibound (indexb (@Build_BoundedIndex string (numQSschemaSchemas DnsSchema)
-                                      (QSschemaNames DnsSchema) sCOLLECTIONS _)).
+                                      (QSschemaNames DnsSchema) sRRecords _)).
 
 Lemma refine_count_constraint_broken' :
   forall (n : resourceRecord) (r : UnConstrQueryStructure DnsSchema),
     refine {b |
             decides b
-                    (forall tup' : @IndexedTuple (GetHeading DnsSchema sCOLLECTIONS),
-                       (GetUnConstrRelation r bCOLLECTIONS) tup' ->
-                       (indexedElement tup')!sNAME = n!sNAME (* switched *)
-                       -> (indexedElement tup')!sTYPE <> CNAME)} (* indexedElement tup', not n *)
+                    (forall tup' : @IndexedTuple (GetHeading DnsSchema sRRecords),
+                        (GetUnConstrRelation r bCOLLECTIONS) tup' ->
+                        (indexedElement tup')!sNAME = n!sNAME (* switched *)
+                        -> (indexedElement tup')!sTYPE <> CNAME)} (* indexedElement tup', not n *)
            (* missing the If/Then statement *)
            (count <- Count
                   For (UnConstrQuery_In r bCOLLECTIONS
@@ -278,30 +280,30 @@ Lemma refine_count_constraint_broken' :
                                            Where (n!sNAME = tup!sNAME
                                                   /\ tup!sTYPE = CNAME ) (* extra /\ condition *)
                                                  Return tup ));
-            ret (beq_nat count 0)).
+              ret (beq_nat count 0)).
 Proof.
   intros; setoid_rewrite refine_forall_to_exists.
   (*refine existence check into query. *)
   match goal with
-      |- context[{b | decides b
-                              (exists tup : @IndexedTuple ?heading,
-                                 (@GetUnConstrRelation ?qs_schema ?qs ?tbl tup /\ @?P tup))}]
-      =>
-      let H1 := fresh in
-      let H2 := fresh in
-      makeEvar (Ensemble (@Tuple heading))
-               ltac:(fun P' => assert (Same_set (@IndexedTuple heading) (fun t => P' (indexedElement t)) P) as H1;
-                     [unfold Same_set, Included, Ensembles.In;
-                       split; [intros x H; pattern (indexedElement x);
-                               match goal with
-                                   |- ?P'' (indexedElement x) => unify P' P'';
-                                     simpl; eauto
-                               end
-                              | eauto]
-                     |
-                     assert (DecideableEnsemble P') as H2;
-                       [ simpl; eauto with typeclass_instances (* Discharge DecideableEnsemble w/ intances. *)
-                       | setoid_rewrite (@refine_constraint_check_into_query' qs_schema tbl qs P P' H2 H1); clear H1 H2 ] ]) end.
+    |- context[{b | decides b
+                            (exists tup : @IndexedTuple ?heading,
+                                (@GetUnConstrRelation ?qs_schema ?qs ?tbl tup /\ @?P tup))}]
+    =>
+    let H1 := fresh in
+    let H2 := fresh in
+    makeEvar (Ensemble (@Tuple heading))
+             ltac:(fun P' => assert (Same_set (@IndexedTuple heading) (fun t => P' (indexedElement t)) P) as H1;
+                             [unfold Same_set, Included, Ensembles.In;
+                              split; [intros x H; pattern (indexedElement x);
+                                      match goal with
+                                        |- ?P'' (indexedElement x) => unify P' P'';
+                                                                      simpl; eauto
+                                      end
+                                     | eauto]
+                             |
+                             assert (DecideableEnsemble P') as H2;
+                             [ simpl; eauto with typeclass_instances (* Discharge DecideableEnsemble w/ intances. *)
+                             | setoid_rewrite (@refine_constraint_check_into_query' qs_schema tbl qs P P' H2 H1); clear H1 H2 ] ]) end.
   (* apply @DecideableEnsemble_And.  apply DecideableEnsemble_EqDec.
   apply Query_eq_list. apply DecideableEnsemble_EqDec. apply Query_eq_RRecordType.
   Print Instances DecideableEnsemble. *)
@@ -311,7 +313,7 @@ Qed.
 
 (* clear_nested_if, using filter_nil_is_nil, clear the nested if/then in honing AddData *)
 Lemma clear_nested_if {A}
-: forall (c c' : bool) (t e e' : A),
+  : forall (c c' : bool) (t e e' : A),
     (c = true -> c' = true)
     -> (if c then (if c' then t else e) else e') = if c then t else e'.
 Proof.
@@ -319,284 +321,157 @@ Proof.
   assert (true = true); [ reflexivity | apply H in H0; discriminate ].
 Qed.
 
-(* if a list is empty, the result of filtering the list with anything will still be empty *)
-Lemma filter_nil_is_nil {A}
-: forall (l : list A) (pred : A -> bool),
-    beq_nat (Datatypes.length l) 0 = true
-    ->  beq_nat (Datatypes.length (filter pred l)) 0 = true.
-Proof.
-  induction l; intros; simpl; try inversion H.
-  reflexivity.
-Qed.
-
-Lemma andb_implication_preserve :
-  forall a b, (a = true -> b = true) -> a = b && a.
-Proof.
-  intros; destruct a; destruct b; symmetry; auto.
-Qed.
-Lemma andb_permute :
-  forall a b c, a && (b && c) = b && (a && c).
-  intros.
-  repeat rewrite andb_assoc.
-  replace (a && b) with (b && a) by apply andb_comm.
-  reflexivity.
-Qed.
-
-    Lemma refine_filtered_list {A}
-    : forall (xs : list A)
-             (P : Ensemble A)
-             (P_dec : DecideableEnsemble P),
-        refine (filtered_list xs P)
-               (ret (filter dec xs)).
-    Proof.
-      unfold filtered_list; induction xs; intros.
-      - reflexivity.
-      - simpl; setoid_rewrite IHxs.
-        simplify with monad laws.
-        destruct (dec a) eqn: eq_dec_a;
-          [ setoid_rewrite dec_decides_P in eq_dec_a; refine pick val true |
-            setoid_rewrite Decides_false in eq_dec_a; refine pick val false ];
-          auto; simplify with monad laws; reflexivity.
-    Qed.
-
-    Definition find_upperbound {A} (f : A -> nat) (ns : list A) : list A :=
-      let max := fold_right
-                   (fun n acc => max (f n) acc) O ns in
-      filter (fun n => NPeano.leb max (f n)) ns.
-
-    Lemma fold_right_max_is_max {A}
-    : forall (f : A -> nat) ns n,
-        List.In n ns -> f n <= fold_right (fun n acc => max (f n) acc) 0 ns.
-    Proof.
-      induction ns; intros; inversion H; subst; simpl;
-      apply NPeano.Nat.max_le_iff; [ left | right ]; auto.
-    Qed.
-
-    Lemma fold_right_higher_is_higher {A}
-    : forall (f : A -> nat) ns x,
-        (forall r, List.In r ns -> f r <= x) ->
-        fold_right (fun n acc => max (f n) acc) 0 ns <= x.
-    Proof.
-      induction ns; simpl; intros; [ apply le_0_n | ].
-      apply NPeano.Nat.max_lub.
-      apply H; left; auto.
-      apply IHns; intros; apply H; right; auto.
-    Qed.
-
-    Lemma find_upperbound_highest_length {A}
-    : forall (f : A -> nat) ns n,
-        List.In n (find_upperbound f ns) -> forall n', List.In n' ns -> (f n) >= (f n').
-    Proof.
-      unfold ge, find_upperbound; intros.
-      apply filter_In in H; destruct H; apply NPeano.leb_le in H1.
-      rewrite <- H1; clear H1 H n.
-      apply fold_right_max_is_max; auto.
-    Qed.
-
-    Instance DecideableEnsembleUpperbound {A} (f : A -> nat) ns :
-      DecideableEnsemble (upperbound f ns) :=
-      {| dec n := NPeano.leb (fold_right (fun n acc => max (f n) acc) O ns) (f n) |}.
-    Proof.
-      unfold upperbound, ge; intros; rewrite NPeano.leb_le; intuition.
-      - remember (f a); clear Heqn; subst; eapply le_trans;
-        [ apply fold_right_max_is_max; apply H0 | assumption ].
-      - eapply fold_right_higher_is_higher; eauto.
-    Defined.
-
-    Corollary refine_find_upperbound {A}
-    : forall (f : A -> nat) ns,
-        refine ([[n in ns | upperbound f ns n]])
-               (ret (find_upperbound f ns)).
-    Proof.
-      intros.
-      setoid_rewrite refine_filtered_list with (P_dec := DecideableEnsembleUpperbound f ns).
-      reflexivity.
-    Qed.
-
-    Lemma eqListA_eq {A}:
-      forall l l0 : list A,
-        SetoidList.eqlistA eq l l0 <-> l = l0.
-    Proof.
-      induction l; split; intros; inversion H; subst; eauto.
-      - f_equal; eapply IHl; eauto.
-      - f_equiv.
-    Qed.
-
-    (* used in refine_check_one_longest_prefix_s and refine_check_one_longest_prefix_CNAME *)
-    Lemma all_longest_prefixes_same :
-      forall (ns : list resourceRecord) (s : list string),
-        (* the name (list string) of every record in the list is a prefix
+(* used in refine_check_one_longest_prefix_s and refine_check_one_longest_prefix_CNAME *)
+Lemma all_longest_prefixes_same :
+  forall (ns : list resourceRecord) (s : list string),
+    (* the name (list string) of every record in the list is a prefix
            of the given name (list string) *)
-        (* e.g. [com.google, com.google.us, com.google.us.scholar] with s = com.google.us.scholar *)
-        (forall (n' : resourceRecord), List.In n' ns -> IsPrefix (get_name n') s)
+    (* e.g. [com.google, com.google.us, com.google.us.scholar] with s = com.google.us.scholar *)
+    (forall (n' : resourceRecord), List.In n' ns -> IsPrefix (get_name n') s)
 
-        (* for two records, if they both have the longest names in the list of records
+    (* for two records, if they both have the longest names in the list of records
            (AND as before, they are prefixes of s)
          then their names must be the same *)
-        -> forall n n' : resourceRecord, List.In n (find_upperbound name_length ns)
-                        -> List.In n' (find_upperbound name_length ns)
-                        -> get_name n = get_name n'.
-    Proof.
-      unfold find_upperbound, name_length; intros ns s H0 n n' H H1.
-      apply filter_In in H; destruct H; apply filter_In in H1; destruct H1.
-      pose proof (H0 _ H); pose proof (H0 _ H1).
-      apply NPeano.leb_le in H2; apply NPeano.leb_le in H3.
-      pose proof (fold_right_max_is_max name_length ns n H) as H2'.
-      pose proof (fold_right_max_is_max name_length ns n' H1) as H3'.
-      unfold name_length in *.
-      apply (le_antisym _ _ H2') in H2; apply (le_antisym _ _ H3') in H3.
-      rewrite <- H2 in H3.
-      unfold IsPrefix in *; destruct H4; destruct H5; rewrite <- H5 in H4.
-      clear H2' H3' H H2 H0 H1 H5 s ns.
-      remember (get_name n); remember (get_name n'); clear Heql Heql0.
-      (* if 2 lists have the same length and are both prefixes of some list, they are the same list *)
-      apply eqListA_eq in H4.
-      revert x0 l l0 H4 H3.
-      induction x; destruct x0; intros.
-      - repeat rewrite app_nil_r in H4; assumption.
-      - apply f_equal with (f := @Datatypes.length string) in H4.
-        repeat rewrite app_length in H4; subst; exfalso; simpl in *; omega.
-      - apply f_equal with (f := @Datatypes.length string) in H4.
-        repeat rewrite app_length in H4; subst; exfalso; simpl in *; omega.
-      - rewrite app_comm_cons' with (As := l) in H4.
-        rewrite app_comm_cons' with (As := l0) in H4.
-        apply IHx in H4; [ apply app_inj_tail in H4; destruct H4; auto |
-        repeat rewrite app_length; rewrite H3; reflexivity ].
-    Qed.
+    -> forall n n' : resourceRecord, List.In n (find_UpperBound name_length ns)
+                                     -> List.In n' (find_UpperBound name_length ns)
+                                     -> get_name n = get_name n'.
+Proof.
+  unfold find_UpperBound, name_length; intros ns s H0 n n' H H1.
+  apply filter_In in H; destruct H; apply filter_In in H1; destruct H1.
+  pose proof (H0 _ H); pose proof (H0 _ H1).
+  apply NPeano.leb_le in H2; apply NPeano.leb_le in H3.
+  pose proof (fold_right_max_is_max name_length ns n H) as H2'.
+  pose proof (fold_right_max_is_max name_length ns n' H1) as H3'.
+  unfold name_length in *.
+  apply (le_antisym _ _ H2') in H2; apply (le_antisym _ _ H3') in H3.
+  rewrite <- H2 in H3.
+  unfold IsPrefix in *; destruct H4; destruct H5; rewrite <- H5 in H4.
+  clear H2' H3' H H2 H0 H1 H5 s ns.
+  remember (get_name n); remember (get_name n'); clear Heqd Heqd0.
+  (* if 2 lists have the same length and are both prefixes of some list, they are the same list *)
+  apply eqListA_eq in H4.
+  revert x0 d d0 H4 H3.
+  induction x; destruct x0; intros.
+  - repeat rewrite app_nil_r in H4; assumption.
+  - apply f_equal with (f := @Datatypes.length string) in H4.
+    repeat rewrite app_length in H4; subst; exfalso; simpl in *; omega.
+  - apply f_equal with (f := @Datatypes.length string) in H4.
+    repeat rewrite app_length in H4; subst; exfalso; simpl in *; omega.
+  - rewrite app_comm_cons' with (As := d1) in H4.
+    rewrite app_comm_cons' with (As := d0) in H4.
+    apply IHx in H4;
+      [ apply (app_inj_tail d0 d1) in H4; destruct H4; auto
+      | repeat rewrite app_length; rewrite H3; reflexivity ].
+Qed.
 
-    Ltac find_if_inside_eqn :=
-      match goal with
-        | [ |- context[if ?X then _ else _] ] => destruct X eqn: ?
-        | [ H : context[if ?X then _ else _] |- _ ]=> destruct X eqn: ?
-      end.
+Ltac find_if_inside_eqn :=
+  match goal with
+  | [ |- context[if ?X then _ else _] ] => destruct X eqn: ?
+  | [ H : context[if ?X then _ else _] |- _ ]=> destruct X eqn: ?
+  end.
 
-    (* ------------------ *)
+(* ------------------ *)
 
-    (* These 3 lemmas relating to prefixes help hone the Process method in DnsManual *)
+(* These 3 lemmas relating to prefixes help hone the Process method in DnsManual *)
 
-    (* Implement the check for an exact match *)
-    (* uses all_longest_prefixes_same *)
-    Lemma refine_check_one_longest_prefix_s
-    : forall (ns : list resourceRecord) (s : list string),
-        (* the name (list string) of every record in the list is a prefix
+(* Implement the check for an exact match *)
+(* uses all_longest_prefixes_same *)
+Lemma refine_check_one_longest_prefix_s
+  : forall (ns : list resourceRecord) (s : list string),
+    (* the name (list string) of every record in the list is a prefix
            of the given name (list string) *)
-        (forall n' : resourceRecord, List.In n' ns -> IsPrefix (get_name n') s) ->
+    (forall n' : resourceRecord, List.In n' ns -> IsPrefix (get_name n') s) ->
 
-        (* there exists no record such that it is one of the longest prefixes of the name
+    (* there exists no record such that it is one of the longest prefixes of the name
            AND is not the name itself -- refines to a computation that just checks the first
            the name against the first longest prefix found. it's ok to just check the first
            due to all_longest_prefixes_same: all longest prefixes must be the same *)
-        refine {b : bool |
-                decides b
-                        (~
-                           (exists x : resourceRecord,
-                              List.In x (find_upperbound name_length ns) /\ s <> (get_name x)))}
+    refine {b : bool |
+            decides b
+                    (~
+                       (exists x : resourceRecord,
+                           List.In x (find_UpperBound name_length ns) /\ s <> (get_name x)))}
 
-               (ret match find_upperbound name_length ns with
-                      | nil => true
-                      | n' :: _ => ?[s == (get_name n')]
-                    end).
-    Proof.
-      computes_to_econstructor; simpl in H; intros; computes_to_inv.
-      subst; unfold decides; pose proof (all_longest_prefixes_same ns H); clear H.
-      remember (find_upperbound name_length ns) as l.
-      unfold If_Then_Else.
-      find_if_inside_eqn.
-      - unfold not; intros; repeat destruct H; apply H1; clear H1; destruct l;
-        [ inversion H | subst; apply H0 with (n := r) in H ];
-        [ find_if_inside; [ subst; auto | inversion Heqb ] | simpl; left; auto ].
-      - unfold not; intros; apply H; clear H; destruct l; try inversion Heqb.
-        exists r; split; [ simpl; left; auto | intros; rewrite <- H in Heqb ].
-        find_if_inside; [ discriminate | unfold not in *; apply n; auto ].
-    Qed.
+           (ret match find_UpperBound name_length ns with
+                | nil => true
+                | n' :: _ => ?[s == (get_name n')]
+                end).
+Proof.
+  computes_to_econstructor; simpl in H; intros; computes_to_inv.
+  subst; unfold decides; pose proof (all_longest_prefixes_same ns H); clear H.
+  remember (find_UpperBound name_length ns) as l.
+  unfold If_Then_Else.
+  find_if_inside_eqn.
+  - unfold not; intros; repeat destruct H; apply H1; clear H1; destruct l;
+      [ inversion H | subst; apply H0 with (n := r) in H ];
+      [ find_if_inside; [ subst; auto | inversion Heqb ] | simpl; left; auto ].
+  - unfold not; intros; apply H; clear H; destruct l; try inversion Heqb.
+    exists r; split; [ simpl; left; auto | intros; rewrite <- H in Heqb ].
+    find_if_inside; [ discriminate | unfold not in *; apply n; auto ].
+Qed.
 
-    Lemma in_list_exists {A}
-    : forall (xs : list A) x, List.In x xs -> exists n, nth_error xs n = Some x.
-    Proof.
-      intros; induction xs; inversion H; subst.
-      exists 0; reflexivity.
-      apply IHxs in H0; destruct_ex; exists (1 + x0); auto.
-    Qed.
+(* uses all_longest_prefixes_same; very similar to refine_check_one_longest_prefix_s but with an extra condition/Tuple type *)
+Lemma refine_check_one_longest_prefix_CNAME
+  : forall (ns : list resourceRecord) (n : RRecordType) (s : list string)
+           (HH : forall (t t' : resourceRecord) (n n' : nat),
+               n <> n'
+               -> nth_error ns n  = Some t
+               -> nth_error ns n' = Some t'
+               -> get_name t      = get_name t'
+               -> t!sTYPE <> CNAME),
+    (* forall HH? *)
 
-    Lemma exists_in_list {A}
-    : forall (xs : list A) x, (exists n, nth_error xs n = Some x) -> List.In x xs.
-    Proof.
-      intros. revert x H.
-      induction xs; intros.
-      - destruct H. destruct x0; inversion H.
-      - simpl in *. destruct H. destruct x0.
-        * left. inversion H. auto.
-        * right. apply IHxs. eexists. apply H.
-    Qed.
-
-    Lemma in_list_preserve_filter {A}
-    : forall (f : A -> bool) xs x, List.In x (filter f xs) -> List.In x xs.
-    Proof.
-      intros; apply (filter_In f x xs) in H; tauto.
-    Qed.
-
-    (* uses all_longest_prefixes_same; very similar to refine_check_one_longest_prefix_s but with an extra condition/Tuple type *)
-    Lemma refine_check_one_longest_prefix_CNAME
-    : forall (ns : list resourceRecord) (n : RRecordType) (s : list string)
-             (HH : forall (t t' : resourceRecord) (n n' : nat),
-                 n <> n'
-                 -> nth_error ns n  = Some t
-                 -> nth_error ns n' = Some t'
-                 -> get_name t      = get_name t'
-                 -> t!sTYPE <> CNAME),
-        (* forall HH? *)
-
-        (* as before, the name (list string) of every record in the list is a prefix
+    (* as before, the name (list string) of every record in the list is a prefix
            of the given name (list string) *)
-        (forall n' : resourceRecord, List.In n' ns -> IsPrefix (get_name n') s) ->
+    (forall n' : resourceRecord, List.In n' ns -> IsPrefix (get_name n') s) ->
 
-        (* Tuple type instead of record?
+    (* Tuple type instead of record?
         all "records" that contain the longest prefixes and are not CNAME, and n isn't CNAME  *)
-        (* this should be generalized to {b | List in ... /\ P} => match (...) with (P first one) *)
-        refine {b' : option Tuple |
-                forall b : Tuple,
-                  b' = Some b <->
-                  List.In b (find_upperbound name_length ns) /\
-                  b!sTYPE = CNAME /\ n <> CNAME}
-               (* refines to just checking the condition (with booleans) on the first longest prefix
+    (* this should be generalized to {b | List in ... /\ P} => match (...) with (P first one) *)
+    refine {b' : option Tuple |
+            forall b : Tuple,
+              b' = Some b <->
+              List.In b (find_UpperBound name_length ns) /\
+              b!sTYPE = CNAME /\ n <> CNAME}
+           (* refines to just checking the condition (with booleans) on the first longest prefix
                 using all_longest_prefixes_same *)
-               (ret match (find_upperbound name_length ns) with
-                      | nil => None
-                      | n' :: _ => if CNAME == (n'!sTYPE)
-                                   then if n == CNAME
-                                        then None
-                                        else Some n'
-                                   else None
-                    end).
-    Proof.
-      unfold refine, not; intros; pose proof (all_longest_prefixes_same ns H); clear H.
-      remember (find_upperbound name_length ns) as l.
-      computes_to_inv; computes_to_econstructor; split; intros.
-      - destruct l; [ subst; inversion H | ].
-        repeat find_if_inside_eqn; subst; try inversion H; subst.
-        repeat split; [ simpl; left | symmetry | ]; auto.
-      - destruct H as [? [? ?] ]; destruct l; [ inversion H | subst ].
-        inversion H; unfold not in *.
-        + repeat find_if_inside; subst; auto; exfalso; auto.
-        + assert (r = b).
-          * pose proof (in_eq r l).
-            pose proof H; rewrite Heql in H5; pose proof (in_list_preserve_filter _ ns b H5); clear H5.
-            pose proof H4; rewrite Heql in H5; pose proof (in_list_preserve_filter _ ns r H5); clear H5.
-            pose proof (in_list_exists ns b H6); pose proof (in_list_exists ns r H7); destruct_ex; pose proof (H1 r b H4 H).
-            destruct (beq_nat x0 x) eqn: eq; [ rewrite beq_nat_true_iff in eq; subst; rewrite H8 in H5; inversion H5; auto | ].
-            rewrite beq_nat_false_iff in eq; symmetry in H9.
-            (* HH instantiated here *)
-            pose proof (HH b r x0 x eq H5 H8 H9); exfalso; auto.
-          * repeat find_if_inside; subst; [ exfalso; apply H3 | | exfalso; apply n0 ]; auto.
-    Qed.
+           (ret match (find_UpperBound name_length ns) with
+                | nil => None
+                | n' :: _ => if CNAME == (n'!sTYPE)
+                             then if n == CNAME
+                                  then None
+                                  else Some n'
+                             else None
+                end).
+Proof.
+  unfold refine, not; intros; pose proof (all_longest_prefixes_same ns H); clear H.
+  remember (find_UpperBound name_length ns) as l.
+  computes_to_inv; computes_to_econstructor; split; intros.
+  - destruct l; [ subst; inversion H | ].
+    repeat find_if_inside_eqn; subst; try inversion H; subst.
+    repeat split; [ simpl; left | symmetry | ]; auto.
+  - destruct H as [? [? ?] ]; destruct l; [ inversion H | subst ].
+    inversion H; unfold not in *.
+    + repeat find_if_inside; subst; auto; exfalso; auto.
+    + assert (r = b).
+      * pose proof (in_eq r l).
+        pose proof H; rewrite Heql in H5; pose proof (in_list_preserve_filter _ ns b H5); clear H5.
+        pose proof H4; rewrite Heql in H5; pose proof (in_list_preserve_filter _ ns r H5); clear H5.
+        pose proof (in_list_exists ns b H6); pose proof (in_list_exists ns r H7); destruct_ex; pose proof (H1 r b H4 H).
+        destruct (beq_nat x0 x) eqn: eq; [ rewrite beq_nat_true_iff in eq; subst; rewrite H8 in H5; inversion H5; auto | ].
+        rewrite beq_nat_false_iff in eq; symmetry in H9.
+        (* HH instantiated here *)
+        pose proof (HH b r x0 x eq H5 H8 H9); exfalso; auto.
+      * repeat find_if_inside; subst; [ exfalso; apply H3 | | exfalso; apply n0 ]; auto.
+Qed.
 
-    Lemma refine_If_Opt_Then_Else_ret {A B} :
-      forall i (t : A -> B) (e : B),
-        refine (@If_Opt_Then_Else A (Comp B) i (fun a => ret (t a)) (ret e))
-               (ret (@If_Opt_Then_Else A B i t e)).
-    Proof.
-      destruct i; reflexivity.
-    Qed.
+Lemma refine_If_Opt_Then_Else_ret {A B} :
+  forall i (t : A -> B) (e : B),
+    refine (@If_Opt_Then_Else A (Comp B) i (fun a => ret (t a)) (ret e))
+           (ret (@If_Opt_Then_Else A B i t e)).
+Proof.
+  destruct i; reflexivity.
+Qed.
 
 Lemma refine_decides_forall_In' :
   forall {A} l (P: A -> Prop) (P_Dec : DecideableEnsemble P),
@@ -614,6 +489,7 @@ Proof.
   destruct H1; intuition.
 Qed.
 
+
 Opaque Query_For.
 
 (* ------------------------------ *)
@@ -629,16 +505,16 @@ Lemma flatmap_permutation : forall heading l1 (l2 : list (@RawTuple heading)),
 Proof.
   intros. revert l1 H.
   induction l2; intros; destruct l1; intros; simpl in *;
-  try reflexivity; inv H; (inv H0; inv H1; inv H0; inv H2; inv H).
+    try reflexivity; inv H; (inv H0; inv H1; inv H0; inv H2; inv H).
   - inv H3.
   - rewrite app_singleton. auto.
 Qed.
 
 Lemma flatmap_permutation' : forall heading (l : list (@RawTuple heading)),
     In _ (@FlattenCompList.flatten_CompList (@RawTuple heading)
-     (@map (@RawTuple heading) (Comp (list (@RawTuple heading)))
-        (fun r : @RawTuple heading => @Query_Return (@RawTuple heading) r) l))
-     l.
+                                            (@map (@RawTuple heading) (Comp (list (@RawTuple heading)))
+                                                  (fun r : @RawTuple heading => @Query_Return (@RawTuple heading) r) l))
+       l.
 Proof.
   intros.
   induction l; simpl. Transparent ret.
@@ -653,86 +529,11 @@ Proof.
       apply In_singleton.
     * exists l.
       split.
-      + auto.
-      + unfold ret.
-        rewrite app_singleton.
-        apply In_singleton.
-        Opaque ret. Opaque Bind.
-Qed.
-
-Definition UnIndexedEnsembleListExists
-           (ElementType : Type) (ensemble : @IndexedEnsemble ElementType) :=
-  exists lIndexed : list (@IndexedElement ElementType),
-    exists lElems : list ElementType,
-      map indexedElement lIndexed = lElems /\
-      (forall x : IndexedElement, In IndexedElement ensemble x <-> List.In x lIndexed) /\
-      NoDup (map elementIndex lIndexed).
-
-Lemma nth_error_map' {A B}
-  : forall (f : A -> B) l m b,
-    nth_error (map f l) m = Some b ->
-    exists a, nth_error l m = Some a /\ f a = b.
-Proof.
-  induction l; destruct m; simpl; intros; try discriminate;
-  injections; eauto.
-Qed.
-
-Lemma unindexed_OK_exists_index' heading :
-  forall x lIndexed (t t' : @Tuple heading) n n',
-      n <> n'
-      -> nth_error x n = Some t
-      -> nth_error x n' = Some t'
-      -> Permutation x (map indexedElement lIndexed)
-      -> exists m m' idx idx',
-          m <> m'
-          /\ nth_error lIndexed m = Some {| elementIndex := idx; indexedElement := t |}
-          /\ nth_error lIndexed m' = Some {| elementIndex := idx'; indexedElement := t' |}.
-Proof.
-  intros.
-  eapply PermutationFacts.permutation_map_base in H2; intuition eauto.
-  destruct_ex; intuition; subst.
-  revert t t' n n' H H0 H1; induction H4; intros.
-  - destruct n; simpl in *; discriminate.
-  - destruct n; destruct n'; simpl in *.
-    + intuition.
-    + assert (exists m', nth_error (map indexedElement l') m' = Some t') by
-          (eapply in_list_exists; rewrite <- H4; eapply exists_in_list; eauto).
-      destruct H2.
-      eapply nth_error_map' in H2; destruct_ex; intuition.
-      injections.
-      eexists 0, (S x0), (elementIndex x), (elementIndex x1); intuition; simpl; eauto.
-      destruct x; eauto.
-      rewrite H3; destruct x1; eauto.
-    + assert (exists m, nth_error (map indexedElement l') m = Some t) by
-          (eapply in_list_exists; rewrite <- H4; eapply exists_in_list; eauto).
-      destruct H2.
-      eapply nth_error_map' in H2; destruct_ex; intuition.
-      injections.
-      eexists (S x0), 0, (elementIndex x1), (elementIndex x); intuition; simpl; eauto.
-      rewrite H3; destruct x1; eauto.
-      destruct x; eauto.
-    + destruct (IHPermutation t t' n n') as [m [m' [idx [idx' ?] ] ] ]; eauto.
-      eexists (S m), (S m'), idx, idx'; simpl; intuition eauto.
-  - eapply nth_error_map' in H0; destruct_ex; intuition.
-    eapply nth_error_map' in H1; destruct_ex; intuition.
-    rewrite <- H3, <- H4; destruct x0; destruct x1; simpl in *.
-    destruct n as [ | [ | n ] ];  destruct n' as [ | [ | n' ] ];
-    injections; simpl in *.
-    + intuition.
-    + eexists 1, 0, _, _; simpl; eauto.
-    + eexists 1, (S (S n')), _, _; simpl; repeat split; try eassumption; omega.
-    + eexists 0, 1, _, _; simpl; eauto.
-    + intuition.
-    + eexists 0, (S (S n')), _, _; simpl; repeat split; try eassumption; omega.
-    + eexists (S (S n)), 1, _, _; simpl; repeat split; try eassumption; omega.
-    + eexists (S (S n)), 0, _, _; simpl; repeat split; try eassumption; omega.
-    + eexists (S (S n)), (S (S n')), _, _; simpl; repeat split; try eassumption; omega.
-  -  destruct (IHPermutation1 _ _ _ _ H H0 H1) as [m [m' [idx [idx' ?] ] ] ];
-    intuition.
-     clear H.
-     eapply IHPermutation2; eauto.
-     eapply map_nth_error with (f := indexedElement) in H2; simpl in *; eauto.
-     eapply map_nth_error with (f := indexedElement) in H5; simpl in *; eauto.
+    + auto.
+    + unfold ret.
+      rewrite app_singleton.
+      apply In_singleton.
+      Opaque ret. Opaque Bind.
 Qed.
 
 Theorem IsPrefix_string_dec :
@@ -749,16 +550,16 @@ Lemma tuples_in_relation_satisfy_constraint_specific :
   forall (a : list RawTuple)
          (n : packet)
          (r_n : QueryStructure DnsSchema),
-(* TODO *)
-    For (r in r_n!sCOLLECTIONS)
+    (* TODO *)
+    For (r in r_n!sRRecords)
         (Where (IsPrefix r!sNAME ((n!"questions"!"qname" ))) (* Where Predicate ... *)
                Return r ) ↝ a ->
-  forall (t t' : resourceRecord) (n0 n' : nat),
-    n0 <> n' ->
-    nth_error a n0 = Some t -> (* this isn't right? *)
-    nth_error a n' = Some t' ->
-    get_name t = get_name t' ->
-    t!sTYPE <> CNAME.
+    forall (t t' : resourceRecord) (n0 n' : nat),
+      n0 <> n' ->
+      nth_error a n0 = Some t -> (* this isn't right? *)
+      nth_error a n' = Some t' ->
+      get_name t = get_name t' ->
+      t!sTYPE <> CNAME.
 Proof.
   intros. inversion H. inv H4.
 
@@ -771,136 +572,136 @@ Proof.
                              Return r )) l
              ->  List.incl x l).
   {
-  (* need to use the main H5 too, with the filter
+    (* need to use the main H5 too, with the filter
 this is because x is a list of tuples that all came from r *)
-  clear t t' n0 H0 H1 H2 H3 H n'.
-  remember H5 as inFilter. clear HeqinFilter H5.
-  intros l inRelation.
-  inversion inFilter.
-  inv H.
-  simpl in *.
+    clear t t' n0 H0 H1 H2 H3 H n'.
+    remember H5 as inFilter. clear HeqinFilter H5.
+    intros l inRelation.
+    inversion inFilter.
+    inv H.
+    simpl in *.
 
-  inv H0.
-  (* H : x0 (new) is x1 without indices, and all indices in x1 are unique, and
-     forall x2 (new) : indexedelement, it's in sCOLLECTIONS if and only if it's in x1, the list of indexed elements  *)
+    inv H0.
+    (* H : x0 (new) is x1 without indices, and all indices in x1 are unique, and
+     forall x2 (new) : indexedelement, it's in sRRecords if and only if it's in x1, the list of indexed elements  *)
 
-  inv H.
-  inv H2.
-  remember (map elementIndex x1) as x0.
+    inv H.
+    inv H2.
+    remember (map elementIndex x1) as x0.
 
-  inversion inRelation.
-  inversion H2. clear H2. inversion H3. clear H3.
-  inversion H2. clear H2. inversion H5. clear H5.
-  simpl in *.             (* TODO ltac for these inversions and reasoning about them *)
+    inversion inRelation.
+    inversion H2. clear H2. inversion H3. clear H3.
+    inversion H2. clear H2. inversion H5. clear H5.
+    simpl in *.             (* TODO ltac for these inversions and reasoning about them *)
 
-  unfold incl.
-  subst. (* optional *)
-
-  intros filterElem filterH.
-  remember (map indexedElement x3) as x3elems.
-
-  assert (exists feIndex,
-     List.In {| elementIndex := feIndex; indexedElement := filterElem |} x1).
-  {
-  remember (map indexedElement x1) as x1elems.
-
-  (* this is the real nub of the proof *)
-  assert (List.incl x x1elems).
-  {
     unfold incl.
-    intros xElem. intro.
-    match type of H1 with
-    | appcontext[map (fun r : @RawTuple ?H => (Where (@?H1 r) _))] =>
-      pose proof (In_flatten_CompList H1) as in_flatten
-    end.
+    subst. (* optional *)
 
-    assert ((exists a' : IndexedElement,
-                 List.In a' x1 /\ indexedElement a' = xElem) -> List.In xElem x1elems).
+    intros filterElem filterH.
+    remember (map indexedElement x3) as x3elems.
+
+    assert (exists feIndex,
+               List.In {| elementIndex := feIndex; indexedElement := filterElem |} x1).
     {
-    intros.
-    inversion H5. clear H5.
-    inversion H8. clear H8.
-    rewrite <- H9.
-    rewrite Heqx1elems.
-    apply in_map_iff.
-    eexists.
-    split.
-    reflexivity.
-    auto. }
+      remember (map indexedElement x1) as x1elems.
 
-    apply H5. clear H5.
+      (* this is the real nub of the proof *)
+      assert (List.incl x x1elems).
+      {
+        unfold incl.
+        intros xElem. intro.
+        match type of H1 with
+        | appcontext[map (fun r : @RawTuple ?H => (Where (@?H1 r) _))] =>
+          pose proof (In_flatten_CompList H1) as in_flatten
+        end.
 
-    eapply in_flatten; eauto using IsPrefix_string_dec.
+        assert ((exists a' : IndexedElement,
+                    List.In a' x1 /\ indexedElement a' = xElem) -> List.In xElem x1elems).
+        {
+          intros.
+          inversion H5. clear H5.
+          inversion H8. clear H8.
+          rewrite <- H9.
+          rewrite Heqx1elems.
+          apply in_map_iff.
+          eexists.
+          split.
+          reflexivity.
+          auto. }
 
-    rewrite Heqx1elems in H1.
-    rewrite List.map_map in H1.
-    unfold In in H1.
-    apply H1.
-  }
+        apply H5. clear H5.
 
-  unfold incl in H3.
-  specialize (H3 filterElem).
+        eapply in_flatten; eauto using IsPrefix_string_dec.
 
-  (* alternate version *)
-  assert (List.In filterElem x1elems ->
-          exists index, List.In {| elementIndex := index; indexedElement := filterElem |} x1).
-  {
-  intros.
-  rewrite Heqx1elems in H5.
-  apply in_map_iff in H5.
-  destruct H5.
-  destruct H5.
+        rewrite Heqx1elems in H1.
+        rewrite List.map_map in H1.
+        unfold In in H1.
+        apply H1.
+      }
 
-  destruct x0.
-  simpl in *.
-  rewrite H5 in H8.
-  exists elementIndex.
-  apply H8. }
+      unfold incl in H3.
+      specialize (H3 filterElem).
 
-  specialize (H3 filterH).
-  specialize (H5 H3).
-  destruct H5 as [index].
-  exists index.
-  apply H5.
-  }
+      (* alternate version *)
+      assert (List.In filterElem x1elems ->
+              exists index, List.In {| elementIndex := index; indexedElement := filterElem |} x1).
+      {
+        intros.
+        rewrite Heqx1elems in H5.
+        apply in_map_iff in H5.
+        destruct H5.
+        destruct H5.
 
-  (* ------------------------ *)
+        destruct x0.
+        simpl in *.
+        rewrite H5 in H8.
+        exists elementIndex.
+        apply H8. }
 
-  destruct H3 as [feIndex].                  (* new *)
+      specialize (H3 filterH).
+      specialize (H5 H3).
+      destruct H5 as [index].
+      exists index.
+      apply H5.
+    }
 
-  remember (Build_IndexedElement feIndex filterElem) as indexedFilterElem.
-  specialize (H2 indexedFilterElem).
-  specialize (H indexedFilterElem).
+    (* ------------------------ *)
 
-  inversion H. clear H.
-  inversion H2. clear H2.
+    destruct H3 as [feIndex].                  (* new *)
 
-  specialize (H8 H3).
-  specialize (H H8).
+    remember (Build_IndexedElement feIndex filterElem) as indexedFilterElem.
+    specialize (H2 indexedFilterElem).
+    specialize (H indexedFilterElem).
 
-  clear H5 H8 H9.
+    inversion H. clear H.
+    inversion H2. clear H2.
 
-  eapply Permutation_in.
-  apply Permutation_sym.
-  apply flatmap_permutation; eauto.
+    specialize (H8 H3).
+    specialize (H H8).
 
-  (* there's probably something I can do with indices to remove this step *)
-  assert (List.In indexedFilterElem x3 -> List.In filterElem (map indexedElement x3)) as H5.
-  { intros.
-    apply in_map_iff.
-    exists indexedFilterElem.
-    split.
-    - rewrite HeqindexedFilterElem. reflexivity.
-    - auto. }
+    clear H5 H8 H9.
 
-  rewrite <- Heqx3elems in *.
-  apply H5. apply H.
- }                              (* ends List.incl x l *)
-(* ------------------------------------------------------------------------------------ *)
+    eapply Permutation_in.
+    apply Permutation_sym.
+    apply flatmap_permutation; eauto.
+
+    (* there's probably something I can do with indices to remove this step *)
+    assert (List.In indexedFilterElem x3 -> List.In filterElem (map indexedElement x3)) as H5.
+    { intros.
+      apply in_map_iff.
+      exists indexedFilterElem.
+      split.
+      - rewrite HeqindexedFilterElem. reflexivity.
+      - auto. }
+
+    rewrite <- Heqx3elems in *.
+    apply H5. apply H.
+  }                              (* ends List.incl x l *)
+  (* ------------------------------------------------------------------------------------ *)
 
   assert (Permutation a x) by (symmetry; apply H6).
 
-(* prove that everything in a is in sCOLLECTIONS *)
+  (* prove that everything in a is in sRRecords *)
   assert (forall l,
              In (list RawTuple)
                 (let qs_schema := DnsSchema in
@@ -908,7 +709,7 @@ this is because x is a list of tuples that all came from r *)
                  Query_In r' bCOLLECTIONS (fun r : RawTuple => Return r)) l ->
              incl a l).
   {
-    (* x \subset sCOLLECTIONS, and Permutation a x *)
+    (* x \subset sRRecords, and Permutation a x *)
     intros allTuplesInRelation inRelation.
 
     unfold incl.
@@ -923,8 +724,8 @@ this is because x is a list of tuples that all came from r *)
     apply H7. auto.
   }
 
-(* use the proof that the constraints hold on everything in sC, therefore on a *)
-(* t and t' are in a, therefore the constraint must hold on them *)
+  (* use the proof that the constraints hold on everything in sC, therefore on a *)
+  (* t and t' are in a, therefore the constraint must hold on them *)
   (* this is the top-level goal  *)
 
   assert (List.In t a).
@@ -943,7 +744,7 @@ this is because x is a list of tuples that all came from r *)
   destruct H5 as [x' [Equiv [Equiv' Equiv''] ] ].
   rewrite <- Equiv in *.
   eapply flatmap_permutation in H5'; rewrite H5' in H7.
-  destruct (unindexed_OK_exists_index' _ _ H0 H1 H2 H7) as [m [m' [idx [idx' ?] ] ] ];
+  destruct (unindexed_OK_exists_index' _ H0 H1 H2 H7) as [m [m' [idx [idx' ?] ] ] ];
     intuition.
 
   pose proof (rawTupleconstr (ith2 (rawRels r_n) (Fin.F1 ))) as
@@ -956,17 +757,17 @@ this is because x is a list of tuples that all came from r *)
   eapply map_nth_error with (f := elementIndex) in H16.
   {
     revert m m' H5 H16 H14 Equiv''; clear; unfold Tuple; simpl; induction (map elementIndex x').
-  - destruct m; destruct m'; simpl; intros; try discriminate.
-  - destruct m; destruct m'; simpl; intros; try discriminate.
-    + intuition.
-    + inversion Equiv''; subst.
-      intro; subst; apply H1; injections; apply exists_in_list; eauto.
-    + inversion Equiv''; subst.
-      intro; subst; apply H1; injections; apply exists_in_list; eauto.
-    + inversion Equiv''; eauto.
-}
+    - destruct m; destruct m'; simpl; intros; try discriminate.
+    - destruct m; destruct m'; simpl; intros; try discriminate.
+      + intuition.
+      + inversion Equiv''; subst.
+        intro; subst; apply H1; injections; apply exists_in_list; eauto.
+      + inversion Equiv''; subst.
+        intro; subst; apply H1; injections; apply exists_in_list; eauto.
+      + inversion Equiv''; eauto.
+  }
 
-assert (List.In {| elementIndex := idx; indexedElement := t |} x').
+  assert (List.In {| elementIndex := idx; indexedElement := t |} x').
   { eapply exists_in_list; eauto. }
   apply Equiv' in H15; destruct H15; apply H15.
   assert (List.In {| elementIndex := idx'; indexedElement := t' |} x').
